verification/Dispose.dfy
@@ -1,13 +1,35 @@
 include "TestedBlood.dfy"
 include "TestedBloodList.dfy"
+include "DisposeBlood.dfy"
+include "DisposeBloodList.dfy"
 
 // check if given blood is exp
-method checkExp(blood: TestedBlood){
-
+// Correspond to Dispose::checkExp()
+predicate checkExp(blood: TestedBlood, timenow: int)
+{
+    blood.expiration < timenow
 }
 
 // go through the list, check if the blood is exp
 // if exp, move from the list
-method dispose(list: TestedBloodList){
-
+// Correspond to Dispose::dispose()
+method dispose(testedlist: TestedBloodList, disposedlist: DisposedList, timenow: int)
+    modifies testedlist;
+    modifies disposedlist;
+    ensures forall blood: blood in testedlist.list ==> blood.expiration > timenow;
+{
+    var i := 0;
+    while (i < testedlist.list.Length)
+        invariant 0 <= i <= testedlist.list.Length;
+        invariant 0 <= j < i ==> testedlist.list[i].expiration > timenow;
+        decreases testedlist.list.Length - i;
+    {
+        if (testedlist.list[i].expiration <= timenow) {
+            var found, blood := testedlist.list.extractBlood(testedlist.list[i].id);
+            var newlydisposed := new DisposeBlood(blood.id);
+            disposedlist.list.addBlood(newlydisposed);
+        } else {
+            i := i + 1;
+        }
+    }
 }
