implementation/autotest/autotest3.1.sh
@@ -1,0 +1,16 @@
+#!/bin/sh
+
+# Move testing directory
+BASEDIR=$(dirname "$0")
+cd $BASEDIR/../
+
+# Test
+echo "Test 3.1 - Tester Test - Fail test"
+# Type N
+echo -e '1\n1\n05/11/2019 12:12\n\nb\n2\n1\n1\n\nb\n2\n1\nN\n\nb\nq\n' | python3 main.py > /dev/null
+if [ $? -ne 0 ]
+then
+    exit 1
+fi
+echo "Test 3.1 passed"
+
