implementation/autotest/autotest4.sh
@@ -7,7 +7,7 @@ cd $BASEDIR/../
 # Test
 echo "Test 4 - Doctor Test"
 # Type all 2 functions
-echo -e '1\n1\n04/11/2021 12:12\n\nb\n2\n1\n1\n\nb\n2\n1\nY\nO\n25/11/2028 15:16\n\n\b\nb\n3\n3\nAA\nO\n\n4\n\n1\n\n2\n1\n\nb\nq\n' | python3 main.py > /dev/null
+echo -e '1\n1\n04/11/2019 12:12\n\nb\n2\n1\n1\n\nb\n2\n1\nY\nO\n25/11/2028 15:16\n\n\b\nb\n3\n3\nAA\nO\n\n4\n\n1\n\n2\n1\n\nb\nq\n' | python3 main.py > /dev/null
 if [ $? -ne 0 ]
 then
     exit 1
